proofs/specs/Sampling.ec
@@ -1,6 +1,6 @@
 require import AllCore IntDiv List.
 from Jasmin require import JByte_array JWord.
-
+require import Array256.
 require import Parameters GFq Rq VecMat Conversion Serialization Symmetric.
 import PolyLVec PolyKVec PolyMat.
 import CDR Round Zq PolyReduceZq BigZMod MLDSAParams.
